update phase 1 invariants

ironfleet/src/Dafny/Distributed/Protocol/RSL/FailureProof/Phase1/Phase1Proof.i.dfy
@@ -2,12 +2,14 @@ include "../TimestampedRslSystem.i.dfy"
 include "../../CommonProof/Constants.i.dfy"
 include "../Common/assumptions.i.dfy"
 include "../Common/definitions.i.dfy"
+include "../Phase2_PostFail/Phase2Proof.i.dfy"
 
 module RslPhase1Proof_i {
 import opened TimestampedRslSystem_i
 import opened CommonProof__Constants_i
 import opened Common_Assumptions
 import opened Common_Definitions
+import P2 = RslPhase2Proof_PostFail_i
 
 
 
@@ -15,8 +17,8 @@ import opened Common_Definitions
 *                                     Assumptions                                        *
 *****************************************************************************************/
 
-predicate P1Assumption(s:TimestampedRslState) {
-    && CommonAssumptions(s)
+predicate P1Assumption(ts:TimestampedRslState, opn:OperationNumber) {
+    && CommonAssumptions(ts)
     && (var nextStep := ts.t_environment.nextStep; 
         nextStep.LEnvStepHostIos? ==>
             && (forall io | io in nextStep.ios :: !io.LIoOpTimeoutReceive?)
@@ -26,23 +28,34 @@ predicate P1Assumption(s:TimestampedRslState) {
     && NewLeaderDoesNotReceiveOld2a2b(ts)
     && NewLeaderDoesNotProposeFurtherOps(ts, opn)
     && LeaderAlwaysOne(ts)
+    && QuorumOf2bPacketsImpliesValue(ts, opn)
     && minD < SelfDelivery < D < 2*minD
     && ProcessPacket > 0
     && SelfDelivery + TimeActionRange(0) < D
 }
 
-predicate LeaderAlwaysOne(s:TimestampedRslState)
-    requires |s.t_replicas| > 2 
+predicate LeaderAlwaysOne(ts:TimestampedRslState)
+    requires |ts.t_replicas| > 2 
 {
-    && s.t_replicas[1].v.replica.proposer.election_state.current_view == Ballot(1, 1)
-    && (forall idx | 2 <= idx < |s.t_replicas| 
-        :: s.t_replicas[idx].v.replica.proposer.current_state == 0)
+    && ts.t_replicas[1].v.replica.proposer.election_state.current_view == Ballot(1, 1)
+    && (forall idx | 2 <= idx < |ts.t_replicas| 
+        :: ts.t_replicas[idx].v.replica.proposer.current_state == 0)
 }
 
-predicate OldLeaderCrashed(s:TimestampedRslState, s':TimestampedRslState)
-    requires |s.t_replicas| > 2 
+predicate OldLeaderCrashed(ts:TimestampedRslState, ts':TimestampedRslState)
+    requires |ts.t_replicas| > 2 
 {
-    forall idx, tios | TimestampedRslNextOneReplica(ps, ps', idx, ios) :: idx != 0
+    forall idx, tios | TimestampedRslNextOneReplica(ts, ts', idx, tios) :: idx != 0
+}
+
+
+predicate QuorumOf2bPacketsImpliesValue(ts:TimestampedRslState, opn:OperationNumber)
+    requires |ts.t_replicas| > 2 
+{
+    var r := ts.t_replicas[1].v.replica;
+    LProposerCanNominateUsingOperationNumber(r.proposer, r.acceptor.log_truncation_point, r.proposer.next_operation_number_to_propose)
+    ==>
+    && P2.AlwaysInvariantP2_RequestSrcAndBatchSize(ts, opn)
 }
 
 
@@ -50,35 +63,40 @@ predicate OldLeaderCrashed(s:TimestampedRslState, s':TimestampedRslState)
 *                                     Invariants                                        *
 *****************************************************************************************/
 
-
+predicate Phase1Invariant(ts:TimestampedRslState, opn:OperationNumber) 
+    requires |ts.t_replicas| > 2
+    requires RslConsistency(ts)
+{
+    && AlwaysInvariantP1(ts, opn)
+    && PacketsBallotInvariant(ts)
+    && Invariant(ts, opn)
+}
 
 
 predicate AlwaysInvariantP1(ts:TimestampedRslState, opn:OperationNumber)
     requires |ts.t_replicas| > 2
+    requires RslConsistency(ts)
 {
     var l := ts.t_replicas[1];
     var r := l.v.replica;
+    // && AlwaysInvariantP1_RequestSrcAndBatchSize(ts, opn)
     && 0 <= ts.t_replicas[1].v.nextActionIndex <= 9
     && ServersAreNotClients(ts)
     && LSetOfMessage1b(ts.t_replicas[1].v.replica.proposer.received_1b_packets)
-    && AlwaysInvariantP1_RequestSrcAndBatchSize(ts, opn)
-    && All1aPackets_BalLeq_Opn(ts, Ballot(1, 1))
-    && All1bPackets_BalLeq_Opn(ts, Ballot(1, 1))
     && All2aPackets_BalLeq_Opn(ts, Ballot(1, 0), opn)
     && All2bPackets_BalLeq_Opn(ts, Ballot(1, 0), opn)
     && (!exists pkt :: pkt in ts.t_environment.sentPackets && IsNew2aPacket(pkt, opn))
     && (!exists pkt :: pkt in ts.t_environment.sentPackets && IsNew2bPacket(pkt, opn))
     && (!exists pkt :: pkt in ts.t_environment.sentPackets && IsNewReplyPacket(ts, pkt))
-    && ts.t_replicas[1].v.replica.proposer.request_queue == []
     && (forall pkt | pkt in ts.undeliveredPackets :: pkt in ts.t_environment.sentPackets)
-    && ts.t_replicas[1].v.replica.learner.unexecuted_learner_state == map[]
-    && ts.t_replicas[1].v.replica.executor.next_op_to_execute == OutstandingOpUnknown()
-    && ts.t_replicas[1].v.replica.proposer.current_view_suspectors == {}
 
+    // Proposer stuff
+    && r.proposer.request_queue == []
+    && r.proposer.election_state.current_view_suspectors == {}
     && r.proposer.current_state == 2
     && r.proposer.election_state.current_view == Ballot(1, 1)
     && r.proposer.max_ballot_i_sent_1a == Ballot(1, 1)
-    && opn == r.proposer.next_operation_number_to_propose
+    && r.proposer.next_operation_number_to_propose == opn
 
     // Learner and Executor states, maintain for phase 2
     && opn == r.executor.ops_complete
@@ -88,55 +106,62 @@ predicate AlwaysInvariantP1(ts:TimestampedRslState, opn:OperationNumber)
 }
 
 
-/* Current identical as in P2 */
-predicate AlwaysInvariantP1_RequestSrcAndBatchSize(ts:TimestampedRslState, opn:OperationNumber)
-    requires |ts.t_replicas| > 2
-    requires LSetOfMessage1b(ts.t_replicas[1].v.replica.proposer.received_1b_packets)
-{   
-    && All2aPackets_BalLeq_Opn(ts, Ballot(1, 0), opn)
-    && All2bPackets_BalLeq_Opn(ts, Ballot(1, 0), opn)
-    && (forall pkt | IsUndelivered_2aPkt(ts, pkt) :: RequestBatchSrcInClientIds(ts, pkt.msg.v.val_2a))
-    && (forall pkt | IsUndelivered_2bPkt(ts, pkt) :: RequestBatchSrcInClientIds(ts, pkt.msg.v.val_2b))
-    && (forall pkt | pkt in ts.t_environment.sentPackets && pkt.msg.v.RslMessage_2a? :: |pkt.msg.v.val_2a| > 0)
-    && (forall pkt | pkt in ts.t_environment.sentPackets && pkt.msg.v.RslMessage_2b? :: |pkt.msg.v.val_2b| > 0)
-    && (forall pkt, opn'| pkt in ts.t_environment.sentPackets && pkt.msg.v.RslMessage_1b? && opn' in pkt.msg.v.votes
-        ::  && |pkt.msg.v.votes[opn'].max_val| > 0
-            && RequestBatchSrcInClientIds(ts, pkt.msg.v.votes[opn'].max_val))
-    && (forall v | LValIsHighestNumberedProposal(v, ts.t_replicas[1].v.replica.proposer.received_1b_packets, opn)
-        :: |v| > 0)
-    // Leader's received_1b_packets
-    && (forall pkt, op | pkt in ts.t_replicas[1].v.replica.proposer.received_1b_packets && pkt.msg.RslMessage_1b? && op in pkt.msg.votes
-        :: RequestBatchSrcInClientIds(ts, pkt.msg.votes[op].max_val))
-    // Acceptors
-    && (forall idx, opn'| 0 <= idx < |ts.t_replicas| && opn' in ts.t_replicas[idx].v.replica.acceptor.votes
-        ::  && |ts.t_replicas[idx].v.replica.acceptor.votes[opn'].max_val| > 0   
-            &&  RequestBatchSrcInClientIds(ts, ts.t_replicas[idx].v.replica.acceptor.votes[opn'].max_val)
-    )
+predicate PacketsBallotInvariant(ts:TimestampedRslState) {
+    forall pkt | pkt in ts.undeliveredPackets :: 
+    if pkt.msg.v.RslMessage_1a? then 
+        pkt.msg.v.bal_1a == Ballot(1, 1)
+    else if pkt.msg.v.RslMessage_1b? then
+        pkt.msg.v.bal_1b == Ballot(1, 1)
 }
 
 
+/* Current identical as in P2 */
+// predicate AlwaysInvariantP1_RequestSrcAndBatchSize(ts:TimestampedRslState, opn:OperationNumber)
+//     requires |ts.t_replicas| > 2
+//     requires LSetOfMessage1b(ts.t_replicas[1].v.replica.proposer.received_1b_packets)
+// {   
+//     && All2aPackets_BalLeq_Opn(ts, Ballot(1, 0), opn)
+//     && All2bPackets_BalLeq_Opn(ts, Ballot(1, 0), opn)
+//     && (forall pkt | IsUndelivered_2aPkt(ts, pkt) :: RequestBatchSrcInClientIds(ts, pkt.msg.v.val_2a))
+//     && (forall pkt | IsUndelivered_2bPkt(ts, pkt) :: RequestBatchSrcInClientIds(ts, pkt.msg.v.val_2b))
+//     && (forall pkt | pkt in ts.t_environment.sentPackets && pkt.msg.v.RslMessage_2a? :: |pkt.msg.v.val_2a| > 0)
+//     && (forall pkt | pkt in ts.t_environment.sentPackets && pkt.msg.v.RslMessage_2b? :: |pkt.msg.v.val_2b| > 0)
+//     && (forall pkt, opn'| pkt in ts.t_environment.sentPackets && pkt.msg.v.RslMessage_1b? && opn' in pkt.msg.v.votes
+//         ::  && |pkt.msg.v.votes[opn'].max_val| > 0
+//             && RequestBatchSrcInClientIds(ts, pkt.msg.v.votes[opn'].max_val))
+//     && (forall v | LValIsHighestNumberedProposal(v, ts.t_replicas[1].v.replica.proposer.received_1b_packets, opn)
+//         :: |v| > 0)
+//     // Leader's received_1b_packets
+//     && (forall pkt, op | pkt in ts.t_replicas[1].v.replica.proposer.received_1b_packets && pkt.msg.RslMessage_1b? && op in pkt.msg.votes
+//         :: RequestBatchSrcInClientIds(ts, pkt.msg.votes[op].max_val))
+//     // Acceptors
+//     && (forall idx, opn'| 0 <= idx < |ts.t_replicas| && opn' in ts.t_replicas[idx].v.replica.acceptor.votes
+//         ::  && |ts.t_replicas[idx].v.replica.acceptor.votes[opn'].max_val| > 0   
+//             &&  RequestBatchSrcInClientIds(ts, ts.t_replicas[idx].v.replica.acceptor.votes[opn'].max_val)
+//     )
+// }
+
+
 // Things that are true before 1a packets are sent out by the leader
-predicate Before_1a_Sent_Invariant(ts:TimestampedRslState, opn:OperationNumber) 
+predicate Invariant(ts:TimestampedRslState, opn:OperationNumber) 
     requires |ts.t_replicas| > 2
     requires RslConsistency(ts)
 {
-    // Timestamp 
-    && TimeLe(l.ts, NewLeaderP1_InitTS)  // TODO
-    // TODO also need timestamp on 1a packets, since these are already sent
-
-    // Network
     var l := ts.t_replicas[1];
     var r := l.v.replica;
-    && All1aPackets_BalLeq_Opn(ts, Ballot(1, 1))
-    && All1bPackets_BalLeq_Opn(ts, Ballot(1, 0))
-    && (forall pkt :: pkt in ts.t_environment.sentPackets && pkt.msg.v.RslMessage_1a? :: IsNew1aPacket(pkt))
-    && (!exists pkt :: pkt in ts.t_environment.sentPackets && IsNew1bPacket(pkt))
+
+    // Timestamps
+    && TimeLe(l.ts, TimeBoundPhase1Leader(l.v.nextActionIndex)) 
+
+    && (forall pkt | pkt in ts.undeliveredPackets && IsNew1aPacket(pkt)
+        :: TimeLe(pkt.msg.ts, TimeBound1aDelivery()))
+
+    && (forall pkt | pkt in ts.undeliveredPackets && IsNew1bPacket(pkt)
+        :: TimeLe(pkt.msg.ts, TimeBound1bDeliveryPost()))
 
     // Proposer
-    && |r.proposer.received_1b_packets| < LMinQuorumSize(s.constants.all.config)
 
-    // Acceptors
-    // TODO: Need quorum of acceptors accepted only opn. Or somehow assume this?
+
 }
 
 
